dtlc.v
@@ -1,0 +1,125 @@
+From Coq Require Import ssreflect ssrfun ssrbool.
+Set Implicit Arguments.
+Unset Strict Implicit.
+Unset Printing Implicit Defensive.
+
+Require Import Arith.PeanoNat.
+Require Import Coq.Lists.List.
+Require Import Relations.Relation_Operators.
+Require Import Relations.Operators_Properties.
+
+Require Import utlc.
+Import LCNotations.
+
+Open Scope lc_scope.
+
+(* We use a uniform approach to terms and types: they both are lambda terms. *)
+
+(* For types we posit a fundamental term representing types. *)
+Axiom typeTp: LC.
+Axiom typeTpClosed: LC.
+
+Hint Resolve typeTpClosed : lc_step_db.
+
+(* and a fundamental term representing function types, i.e. funTp A B represents the function type A => B. *)
+Axiom funTp : LC.
+Axiom funTpClosed : closed funTp.
+
+Hint Resolve funTpClosed : lc_step_db.
+
+Notation "A '=>' B" := (funTp A B) (at level 60, right associativity).
+
+(* with de Bruijn indices our context just needs to be a list of types *)
+Definition TpCtx := list LC.
+
+(* colon instead of 'of' didn't work *)
+Reserved Notation "Gamma '|-' s 'of' t" (at level 65).
+
+Inductive TpJudgement : TpCtx -> LC -> LC -> Prop :=
+  | tpOfType: forall ctx tp, ctx |- tp of typeTp
+
+  | tpOfVar: forall ctx n tp,
+
+       nth_error ctx n = Some tp
+    -> ctx |- (#n) of tp
+
+  | tpOfApp: forall ctx s t A B,
+
+       ctx |- s of (A => B)
+    -> ctx |- t of A
+    -> ctx |- (s t) of B
+
+  | tpOfLam: forall ctx t A B B',
+       variablesUpticked B B'
+    -> (cons A ctx) |- t of B'
+    -> ctx |- (\ t) of (A => B)
+
+  | eqTp: forall ctx t A B,
+       A <-->* B
+    -> ctx |- t of A
+    -> ctx |- t of B
+
+  | depTp: forall ctx t depTp,
+       (forall tpInstance, closed tpInstance -> ctx |- t of ((\ depTp) tpInstance))
+    -> ctx |- t of (\ depTp)
+
+
+where "Gamma '|-' s 'of' t" := (TpJudgement Gamma s t).
+
+Notation "'|-' s 'of' t" := (nil |- s of t) (at level 65).
+
+Example identityTypeExtensional: forall A, closed A -> |- (\ #0) of (A => A).
+Proof.
+  move => ? ?.
+  by apply: tpOfLam; [apply: ClosedTermsStableUnderUpticking|constructor].
+Qed.
+
+Example identityTypeIntensional: |- (\ #0) of (\ #0 => #0).
+Proof.
+  apply: depTp.
+  move => ? ?.
+  apply: eqTp.
+  - by apply: rst_sym; do ! constructor; auto with lc_step_db.
+  - by apply: identityTypeExtensional.
+Qed.
+
+Definition lc_product_type := \ \ \ (#2) => (#1) => (#0).
+
+
+Example lc_pair_type: |- lc_pair of (\ \ #1 => #0 => lc_product_type (#1) (#0)).
+Proof.
+  have abc: (closed lc_product_type). admit.
+  apply: depTp => ? ?.
+  apply: eqTp.
+  - by apply: rst_sym; do ! constructor; auto with lc_step_db.
+  - apply: eqTp. 
+    + apply: rst_sym. do ! constructor; auto with lc_step_db.
+      econstructor.
+      * by apply: ClosedTermsStableUnderUpticking.
+      * do ! constructor.
+        ** by apply: NClosedTermsStableUnderNSubstitution; auto with lc_step_db.
+        ** by apply: NClosedTermsStableUnderNSubstitution; auto with lc_step_db.
+        ** apply: NClosedTermsStableUnderNSubstitution; auto with lc_step_db.
+    + do ! constructor => ? ?.
+      apply: eqTp.
+      * apply: rst_sym. do ! constructor; auto with lc_step_db.
+      * do ! constructor.
+
+Definition lc_list_type := \ #0 => (#0 => #0) => #0.
+Definition lc_list_type_for (A: LC) := A => (A => A) => A.
+
+Example lc_nil_type: |- lc_nil of lc_list_type.
+Proof.
+  apply: depTp => ? ?.
+  apply: eqTp.
+  - by apply: rst_sym; do ! constructor; auto with lc_step_db.
+  - do ! constructor.
+Qed.
+
+Example lc_cons_type: |- lc_cons of (\ #0 => lc_list_type_for (#0) => lc_list_type_for (#0)).
+Proof.
+  apply: depTp => A ?.
+  apply: eqTp.
+  - by apply: rst_sym; do ! constructor; auto with lc_step_db.
+  - do ! constructor.
+Qed.
