README.md
@@ -4,9 +4,10 @@
 
 With this project, I try to brush up my Coq knowledge and learn more about how de Bruijn indices are implemented. Last time, in [my formalization of a basic ontology language](https://github.com/ComFreek/basic-ontology-language) I learned the hard way that named variables are perhaps not that easy as on pen & paper. Hence, this time I am trying de Bruijn indices from the start.
 
-We start off easy with
+In `utlc.v` we start off pretty easy with
 
 ```coq
+(* Untyped LC (UTLC) *)
 Inductive LC :=
   | var: nat -> LC
   | app: LC -> LC -> LC
@@ -16,9 +17,12 @@ Inductive LC :=
 
 Then, we
 
-- formalize the notion of closed terms and beta reduction,
-- prove `forall s t, (\ \ #1) s t -->* s` (sanity check!),
-- define an internalization `[[-]]` of Coq-level lambda terms into lambda-level terms (Church encoding),
-- and finally define an evaluator term `f` such that `f [[x]] -->* x`.
+- formalize the notions of closed terms and beta reduction (e.g. to prove `forall s t, (\ \ #1) s t -->* s`),
+- define an internalization `[[-]]` of Coq-level lambda terms into lambda-level terms (Church encoding) and subsequently define an evaluator term `f` such that `f [[x]] -->* x`,
+- and in `dtlc.v` (*dependently typed LC*) define a type system.
 
 The evaluator is due <insert other person's name here after I received permission to do so>.
+
+## Status
+
+In development. Suggestions welcome!
